src/simple-proof/Canonical_forms3.v
@@ -17,7 +17,7 @@ Lemma sigma_binds_to_store_binds_raw: forall sto G S l T,
   exists S1 S2,
     S = S1 & (l ~ T) & S2 /\
     exists x,
-      bindsM l x sto /\
+      bindsM l (Some x) sto /\
       G, S |- trm_var (avar_f x) : T.
 Proof.
   introv Wt. generalize l T. induction Wt; introv Bi.
@@ -67,8 +67,8 @@ Qed.
 Lemma sigma_binds_to_store_binds_typing: forall G S sto l T,
   G, S |~ sto ->
   binds l T S ->
-  exists x, 
-    bindsM l x sto /\
+  exists x,
+    bindsM l (Some x) sto /\
     G, S |- trm_var (avar_f x) : T.
 Proof.
   introv Hwf Bi.
@@ -78,11 +78,197 @@ Proof.
 Qed.
 
 Lemma ref_binds_typ: forall G S l T,
-  G, S |-! trm_val (val_loc l) : typ_ref T ->
+  G, S |-! trm_val (val_loc l) : typ_nref T ->
   binds l T S.
 Proof.
   introv Hty.
   inversion Hty. assumption.
+Qed.
+
+Lemma loc_ref: forall G S v T,
+    inert G ->
+    G, S |-# (trm_val v) : typ_ref T ->
+    False.
+Proof.
+  introv Hin H. pose proof (invertible_typing_lemma_v Hin H). dependent induction H0. inversions H0.
+Qed.
+
+Lemma binds_bindsM: forall G S sta sto l x T,
+    inert G ->
+    well_formed G S sta sto ->
+    binds l T S ->
+    bindsM l (Some x) sto ->
+    G, S |- trm_var (avar_f x) : T.
+Proof.
+  introv Hin Hwf HS Hsto. induction Hwf.
+  - false* binds_empty_inv.
+  - pose proof (inert_ok Hin) as OkG. 
+    assert (Hin': inert G). {
+      inversions Hin.
+      - false* empty_push_inv.
+      - destruct (eq_push_inv H2) as [_ [_ ?]]. subst. assumption.
+    }
+    apply* weaken_ty_trm_ctx. 
+  - pose proof (inert_ok Hin) as OkG. 
+    assert (Hin': inert G). {
+      inversions Hin.
+      - false* empty_push_inv.
+      - destruct (eq_push_inv H3) as [_ [_ ?]]. subst. assumption.
+    }
+    apply* weaken_ty_trm_ctx. 
+  - destruct (classicT (l = l0)); subst.
+    + apply binds_update_eq_inv in Hsto. inversion Hsto.
+    + pose proof (binds_update_neq_inv Hsto n). 
+      pose proof (binds_push_neq_inv HS n).
+      apply* weaken_ty_trm_sigma. 
+  - destruct (classicT (l = l0)); subst.
+    + pose proof (binds_update_eq_inv Hsto) as Hsto'. inversions Hsto'.
+      apply (binds_func HS) in H. subst*.
+    + pose proof (binds_update_neq_inv Hsto n). apply* IHHwf.
+Qed.
+
+Lemma test_bindsM: forall G S sta sto l x,
+    inert G ->
+    well_formed G S sta sto ->
+    bindsM l x sto ->
+    l # S ->
+    False.
+Proof.
+  introv Hin Hwf Hb Hnotin. 
+  induction Hwf.
+  - admit.
+  - admit.
+  - admit.
+  - destruct (classicT (l = l0)).
+    + subst. false (fresh_push_eq_inv Hnotin).
+    + pose proof (binds_update_neq_inv Hb n).
+      apply* IHHwf.
+  - destruct (classicT (l = l0)).
+    + subst. false (binds_fresh_inv H Hnotin).
+    + pose proof (binds_update_neq_inv Hb n).
+      apply* IHHwf.
+Qed.
+
+Lemma test_binds_l_notin_ref: forall G S sta sto l x T,
+    inert G ->
+    well_formed G S sta sto ->
+    l # S ->
+    binds x (typ_ref T) G ->
+    binds x (val_loc l) sta ->
+    False.
+Proof.
+  introv Hin Hwf Hnotin HG Hsta. dependent induction Hwf.
+  - false* binds_empty_inv.
+  - assert (Hin': inert G). {
+      inversions Hin.
+      - false* empty_push_inv.
+      - destruct (eq_push_inv H2) as [_ [_ ?]]. subst. assumption.
+    }
+    destruct (classicT (x = x0)).
+    + subst. 
+      apply binds_push_eq_inv in HG. subst. 
+      apply binds_push_eq_inv in Hsta. subst.
+      apply (general_to_tight_typing Hin') in H1. 
+      false* loc_ref.
+    + pose proof (binds_push_neq_inv HG n) as HG'.
+      pose proof (binds_push_neq_inv Hsta n) as Hsta'.
+      apply* IHHwf.
+  - assert (Hin': inert G). {
+      inversions Hin.
+      - false* empty_push_inv.
+      - destruct (eq_push_inv H3) as [_ [_ ?]]. subst. assumption.
+    }
+    destruct (classicT (x = x0)).
+    + subst. clear IHHwf.
+      apply binds_push_eq_inv in HG. inversions HG. 
+      apply binds_push_eq_inv in Hsta. inversions Hsta. 
+      false (test_bindsM Hin' Hwf H1 Hnotin).
+    + pose proof (binds_push_neq_inv HG n) as HG'.
+      pose proof (binds_push_neq_inv Hsta n) as Hsta'.
+      apply* IHHwf.
+  - destruct (classicT (l = l0)).
+    + subst. false (fresh_push_eq_inv Hnotin).
+    + apply* IHHwf. 
+  - destruct (classicT (l = l0)).
+    + subst. false (binds_fresh_inv H Hnotin).
+    + apply* IHHwf.
+Qed.
+
+Lemma test: forall G S sta sto x l T T',
+    inert G ->
+    well_formed G S sta sto ->
+    binds x (typ_ref T) G ->
+    binds l T' S ->
+    binds x (val_loc l) sta ->
+    G, S |- T <: T' ->
+    G, S |- T' <: T ->
+    (* exists S1 S2,  *)
+    (*   S = S1 & (l ~ T) & S2 ->  *)
+      exists y,
+        bindsM l (Some y) sto /\
+        G, S |- trm_var (avar_f y) : T.
+Proof.
+  introv Hin Hwf. gen x l. induction Hwf; introv HG HS Hsta Hs1 Hs2.
+  - false* binds_empty_inv.
+  - pose proof (wf_to_ok_S Hwf) as HokS.
+    assert (Hin': inert G). {
+      inversions Hin.
+      - false* empty_push_inv.
+      - destruct (eq_push_inv H2) as [_ [_ ?]]. subst. assumption.
+    }
+    destruct (classicT (x = x0)).
+    + subst. clear IHHwf. apply binds_push_eq_inv in HG. subst.
+      apply (general_to_tight_typing Hin') in H1.
+      false (loc_ref Hin' H1).
+    + apply neq_sym in n. 
+      pose proof (binds_push_neq_inv HG n) as HG'.
+      pose proof (binds_push_neq_inv Hsta n) as Hsta'.
+      specialize (IHHwf Hin' x0 l HG' HS Hsta').
+      destruct IHHwf as [y [Bi Ht]].
+      exists y. split. 
+      * assumption.
+      * apply* weaken_ty_trm_ctx.
+  - pose proof (wf_to_ok_S Hwf) as HokS.
+    assert (Hin': inert G). {
+      inversions Hin.
+      - false* empty_push_inv.
+      - destruct (eq_push_inv H3) as [_ [_ ?]]. subst. assumption.
+    }
+    destruct (classicT (x = x0)).
+    + subst. clear IHHwf.
+      apply binds_push_eq_inv in HG. inversions HG. 
+      apply binds_push_eq_inv in Hsta. inversions Hsta. 
+      pose proof (binds_bindsM Hin' Hwf HS H1).
+      exists y. split.
+      * assumption.
+      * apply* weaken_ty_trm_ctx.
+    + apply neq_sym in n. 
+      pose proof (binds_push_neq_inv HG n) as HG'.
+      pose proof (binds_push_neq_inv Hsta n) as Hsta'.
+      specialize (IHHwf Hin' x0 l0 HG' HS Hsta').
+      destruct IHHwf as [y' [Bi Ht]].
+      exists y'. split. 
+      * assumption.
+      * apply* weaken_ty_trm_ctx.
+  - pose proof (wf_to_ok_S Hwf) as HokS.
+    destruct (classicT (l = l0)).
+    + subst. apply binds_push_eq_inv in HS. subst. 
+      false (test_binds_l_notin_ref Hin Hwf H HG Hsta).
+    + apply neq_sym in n.
+      pose proof (binds_push_neq_inv HS n) as HS'. 
+      specialize (IHHwf Hin x l0 HG HS' Hsta).
+      destruct IHHwf as [y [Bi Ht]]. exists y. split.
+      * apply* binds_update_neq.
+      * apply* weaken_ty_trm_sigma.
+  - pose proof (wf_to_ok_S Hwf) as HokS.
+    destruct (classicT (l = l0)).
+    + subst. exists x. split. 
+      * apply binds_update_eq.
+      * apply (binds_func HS) in H. subst. assumption.
+    + specialize (IHHwf Hin x0 l0 HG HS Hsta).
+      destruct IHHwf as [y [Bi Ht]]. exists y. split.
+      * apply* binds_update_neq.
+      * assumption.
 Qed.
 
 (*
@@ -96,44 +282,65 @@ If G, S ~ stack, G, S ~ store, G inert, and G, S |- x: Ref T then
 
 Lemma canonical_forms_3: forall G S sta sto x T,
   inert G ->
-  G, S ~~ sta ->
-  G, S |~ sto ->
+  well_formed G S sta sto ->
   G, S |- trm_var (avar_f x) : typ_ref T ->
   exists l y,
     binds x (val_loc l) sta /\
-    G, S |- trm_val (val_loc l) : typ_ref T /\
-    bindsM l y sto /\
+    G, S |- trm_val (val_loc l) : typ_nref T /\
+    bindsM l (Some y) sto /\
     G, S |- trm_var (avar_f y) : T.
 Proof.
-  introv Hg Hwf Hwt Hty.
+  introv Hin Hwf Hty.
   pose proof (typing_implies_bound Hty) as [V Bi].
-  pose proof (general_to_tight_typing Hg Hty) as Hty'.
-  pose proof (invertible_typing_lemma Hg Hty') as Hinv.
-  pose proof (invertible_to_precise_typ_ref Hg Hinv) as [T' [Hx [Hs1 Hs2]]].
-  pose proof (corresponding_types Hwf Hg Bi)
+  pose proof (general_to_tight_typing Hin Hty) as Hty'.
+  pose proof (invertible_typing_lemma Hin Hty') as Hinv.
+  pose proof (invertible_to_precise_typ_ref Hin Hinv) as [T' [Hx [Hs1 Hs2]]].
+  pose proof (corresponding_types Hwf Hin Bi)
     as [[L [U [W [S1 [W1 [t [Hb [Ht [Heq _]]]]]]]]] | [[U [ds [Hb [Ht Heq]]]] | [U [U' [l [Hb [Ht [Heq [Hs1' Hs2']]]]]]]]].
   - assert (H: exists T, record_type T /\ V = (typ_bnd T)).
-    { pose proof (binds_inert Bi Hg) as Hgt.
-      induction Hgt.
+    { pose proof (binds_inert Bi Hin) as HinT.
+      induction HinT.
       - destruct (precise_flow_lemma Hx) as [W' H].
         pose proof (pf_binds H). apply (binds_func Bi) in H0.
         apply pf_inert_ref_U in H. subst. inversion H0. assumption.
       - exists T0. auto.
       - inversion Heq. 
+      - inversion Heq.
     }
     destruct H as [T0 [Hrt Hsubst]]; subst V; rename T0 into V.
     inversion Hsubst.
-  - pose proof (binds_inert Bi Hg) as Hgt.
+  - pose proof (binds_inert Bi Hin) as Hgt.
     induction Hgt.
     + inversion Heq.
     + pose proof (precise_flow_lemma Hx) as [W' H'].
       pose proof (pf_binds H'). apply (binds_func Bi) in H0.
       apply pf_inert_ref_U in H'. subst. inversion H0. assumption.
     + inversion Heq.
+    + inversion Heq.
   - subst. 
     remember Ht as Ht'. inversions Ht'. 
-    pose proof (sigma_binds_to_store_binds_typing Hwt H3) as [y [Bil' Htyl]].
-    pose proof (precise_flow_lemma Hx) as [W' H].
+    destruct Heq; subst. {
+      pose proof (precise_flow_lemma Hx).
+      destruct H as [V Hpf]. pose proof (pf_inert_ref_U Hin Hpf). subst.
+      apply pf_binds in Hpf. apply (binds_func Hpf) in Bi. 
+      inversion Bi.
+    } 
+    {
+      
+      exists l y. repeat split; try assumption.
+      - admit. (* hm *)
+      - admit. (* hm *)
+      - 
+      
+
+      inversions Ht.
+      pose proof (test Hin Hwf Bi H3 Hb) as [y [Bil' Htyl]].
+      pose proof (precise_flow_lemma Hx) as [W' H].
+      destruct Heq; subst.
+    + 
+
+
+
     exists l y. repeat split; try assumption.
     + apply ty_sub with (T:=typ_ref T'). 
       * apply ty_sub with (T:=typ_ref U). 
